whites -> white

tarjan_num.v
@@ -119,10 +119,10 @@ Fact gray_key : unit. Proof tt.
 Definition gray := locked_with gray_key gray_def.
 Lemma grayE : gray = gray_def. Proof. exact: unlock. Qed.
 
-Notation whites_def := (fun e => ~: (gray e :|: black e)).
+Notation white_def := (fun e => ~: (gray e :|: black e)).
 Fact white_key : unit. Proof tt.
-Definition whites := locked_with white_key whites_def.
-Lemma whitesE : whites = whites_def. Proof. exact: unlock. Qed.
+Definition white := locked_with white_key white_def.
+Lemma whiteE : white = white_def. Proof. exact: unlock. Qed.
 
 End other_colors.
 
@@ -134,36 +134,36 @@ Proof.
 by apply/setP=> x; rewrite !inE; apply/negP=> /bigcupP[?]; rewrite inE.
 Qed.
 
-Lemma whites_blackF x e : x \in whites e -> x \in black e = false.
-Proof. by rewrite whitesE grayE !inE; case: (x \in black _). Qed.
+Lemma white_blackF x e : x \in white e -> x \in black e = false.
+Proof. by rewrite whiteE grayE !inE; case: (x \in black _). Qed.
 
-Lemma whites_stackF x e : x \in whites e -> x \in stack e = false.
+Lemma white_stackF x e : x \in white e -> x \in stack e = false.
 Proof.
-by rewrite whitesE grayE !inE andbC; case: (x \in stack _); rewrite //= orNb.
+by rewrite whiteE grayE !inE andbC; case: (x \in stack _); rewrite //= orNb.
 Qed.
 
-Lemma whites_grayF x e : x \in whites e -> x \in gray e = false.
-Proof. by rewrite whitesE !inE; case: (x \in gray e). Qed.
+Lemma white_grayF x e : x \in white e -> x \in gray e = false.
+Proof. by rewrite whiteE !inE; case: (x \in gray e). Qed.
 
 Lemma gray_stack x e : x \in gray e -> x \in stack e.
 Proof. by rewrite grayE !inE andbC; case: (x \in stack _). Qed.
 
-Lemma stack_whitesF x e : x \in stack e -> x \in whites e = false.
-Proof. by rewrite whitesE grayE !inE => ->; case: (_ \in _). Qed.
+Lemma stack_whiteF x e : x \in stack e -> x \in white e = false.
+Proof. by rewrite whiteE grayE !inE => ->; case: (_ \in _). Qed.
 
-Lemma black_whitesF x e : x \in black e -> x \in whites e = false.
-Proof. by rewrite whitesE grayE !inE => ->. Qed.
+Lemma black_whiteF x e : x \in black e -> x \in white e = false.
+Proof. by rewrite whiteE grayE !inE => ->. Qed.
 
-Lemma whites_add_stack x e : whites (add_stack x e) = whites e :\ x.
+Lemma white_add_stack x e : white (add_stack x e) = white e :\ x.
 Proof.
-apply/setP=> y; rewrite whitesE grayE !inE /=.
+apply/setP=> y; rewrite whiteE grayE !inE /=.
 by case: (_ \in _) (_ \in _) (_ == _) => [] [] [].
 Qed.
 
-Lemma gray_add_stack x e : x \in whites e ->
+Lemma gray_add_stack x e : x \in white e ->
   gray (add_stack x e) = x |: gray e.
 Proof.
-move=> x_whites; apply/setP=> y; move: x_whites; rewrite whitesE grayE !inE.
+move=> x_white; apply/setP=> y; move: x_white; rewrite whiteE grayE !inE.
 by case: eqP => [->|]; case: (_ \in _) (_ \in _)=> [] [].
 Qed.
 
@@ -173,9 +173,9 @@ Proof. by []. Qed.
 Lemma gray_add_black e x : gray (add_black x e) = gray e :\ x.
 Proof. by apply/setP=> y; rewrite grayE !inE /= negb_or andbA. Qed.
 
-Lemma whites_add_black e x : whites (add_black x e) = whites e :\ x.
+Lemma white_add_black e x : white (add_black x e) = white e :\ x.
 Proof.
-rewrite whitesE gray_add_black /=; apply/setP=> y; rewrite !inE.
+rewrite whiteE gray_add_black /=; apply/setP=> y; rewrite !inE.
 by case: (_ == _) (_ \in _) (_ \in _) => [] [].
 Qed.
 
@@ -193,12 +193,12 @@ have [|yNs' neq_yx] //= := boolP (y \in s').
 by have [y_s|] //= := boolP (y \in s); rewrite (subsetP sb).
 Qed.
 
-Lemma whites_add_sccs e x :
+Lemma white_add_sccs e x :
   let s := take (index x (stack e)) (stack e) in
   x \in gray e -> uniq (stack e) -> s \subset black e ->
-  whites (add_sccs x e) = whites e.
+  white (add_sccs x e) = white e.
 Proof.
-move=> /= x_gray se_uniq sb; rewrite whitesE gray_add_sccs //=.
+move=> /= x_gray se_uniq sb; rewrite whiteE gray_add_sccs //=.
 by rewrite setUCA setUA setD1K.
 Qed.
 
@@ -231,22 +231,22 @@ Inductive color4_spec x e : bool -> bool -> bool -> bool -> bool -> Type :=
 | Color4Gray of x \in gray e : color4_spec x e false true false true false
 | Color4Sccs of x \in cover (sccs e) :
                        color4_spec x e true false true false false
-| Color4White of x \in whites e : color4_spec x e false false false false true
+| Color4White of x \in white e : color4_spec x e false false false false true
 | Color4BlackStack of x \in black e & x \in stack e :
                         color4_spec x e true true false false false.
 
 Lemma color4P x e : wf_color e ->
                    color4_spec x e (x \in black e) (x \in stack e)
                               (x \in cover (sccs e))
-                              (x \in gray e) (x \in whites e).
+                              (x \in gray e) (x \in white e).
 Proof.
 move=> [/(_ x) s_def /subsetP /(_ x) /implyP].
-move: s_def; rewrite whitesE grayE !inE.
+move: s_def; rewrite whiteE grayE !inE.
 case x_black: (_ \in black _) => /=;
 case x_stack : (_ \in stack _) => /=;
 case x_sccs : (_ \in cover _) => //=; do ?by constructor.
   by constructor=> //; rewrite grayE !inE x_black.
-by constructor; rewrite whitesE grayE !inE x_black x_stack.
+by constructor; rewrite whiteE grayE !inE x_black x_stack.
 Qed.
 
 Lemma stack_sccsF x e : wf_color e -> x \in stack e ->
@@ -268,10 +268,10 @@ Proof. by case/color4P. Qed.
 Lemma sccs_black x e : wf_color e -> x \in cover (sccs e) -> x \in black e.
 Proof. by case/color4P. Qed.
 
-Lemma add_stack_cwf x e : x \in whites e -> wf_color e -> wf_color (add_stack x e).
+Lemma add_stack_cwf x e : x \in white e -> wf_color e -> wf_color (add_stack x e).
 Proof.
 move=> x_white e_wf; split=> /=; do ?
-  by [exact: wf_sccs|rewrite whites_stackF ?wf_uniq].
+  by [exact: wf_sccs|rewrite white_stackF ?wf_uniq].
 move=> y; rewrite gray_add_stack // !inE.
 by case: (_ == _) color4P => [] [].
 Qed.
@@ -311,14 +311,14 @@ by move=> s1 s2 s_uniq y_in; apply: uniq_catRL.
 Qed.
 
 Inductive stack_spec x e : bool -> bool -> bool -> bool -> bool -> Type :=
-| StackWhite of x \in whites e : stack_spec x e true false false false false
+| StackWhite of x \in white e : stack_spec x e true false false false false
 | StackStack of x \in stack e :
                        stack_spec x e false true false (x \in gray e) (x \in black e)
 | StackSccs  of x \in cover (sccs e) :
                         stack_spec x e false false true false true.
 
 Lemma stackP x e : wf_color e ->
-  stack_spec x e (x \in whites e) (x \in stack e) (x \in cover (sccs e))
+  stack_spec x e (x \in white e) (x \in stack e) (x \in cover (sccs e))
                               (x \in gray e) (x \in black e).
 Proof.
 move=> e_cwf; set xb := x \in black _; set xg := x \in gray e.
@@ -353,7 +353,7 @@ Local Notation "x '<[' e ']=' y" := (precedes x y e)
   (at level 10, format "x  '<[' e ]=  y").
 
 Record wf_num e := WfNum {
-   wf_num0      : forall x, (num e x == 0) = (x \in whites e);
+   wf_num0      : forall x, (num e x == 0) = (x \in white e);
    wf_num_infty : forall x, (num e x == infty) = (x \in cover (sccs e));
    wf_num_lt    : forall x, num e x != infty -> num e x < sn e;
    wf_sn        : sn e = #|gray e :|: black e|.+1;
@@ -385,13 +385,13 @@ move=> e_cwf e_nwf; symmetry; rewrite lt0n wf_num0//; case: stackP => //=.
 by rewrite -wf_num_infty => // /eqP->; rewrite ltnNge sn_small.
 Qed.
 
-Lemma add_stack_nwf x e : x \in whites e -> wf_color e ->
+Lemma add_stack_nwf x e : x \in white e -> wf_color e ->
   wf_num e -> wf_num (add_stack x e).
 Proof.
 move=> x_w wf_c wf_e.
 have [nEw nEc nLs snE pE] := wf_e.
 split => [y|y|y||y z]; rewrite ?ffunE ?inE /=.
-- rewrite whites_add_stack; case: (y =P x) => [->|/eqP yDx]; rewrite !inE.
+- rewrite white_add_stack; case: (y =P x) => [->|/eqP yDx]; rewrite !inE.
     by rewrite snE eqxx.
   by rewrite nEw (negPf yDx).
 - case: (y =P x) => [->|//].
@@ -418,7 +418,7 @@ Proof.
 move=> x_g wf_c wf_e.
 have [nEw nEc nLs snE pE] := wf_e.
 split => //= [y|].
-  by rewrite whites_add_black !inE nEw; case: eqP => // ->; case: color4P x_g.
+  by rewrite white_add_black !inE nEw; case: eqP => // ->; case: color4P x_g.
 by rewrite gray_add_black setUA /= [_ :|: [set x]]setUC setD1K.
 Qed.
 
@@ -430,7 +430,7 @@ Proof.
 move=> tsb x_g wf_c wf_n.
 have [nEw nEc nLs snE pE] := wf_n.
 split => [y|y|y||y z]; rewrite ?ffunE ?(inE) /=.
-- rewrite whites_add_sccs ?wf_uniq // mem_rcons inE.
+- rewrite white_add_sccs ?wf_uniq // mem_rcons inE.
   case: (y =P x)=> [->|_] /=; first by case: color4P x_g.
   case: (boolP (_ \in _))=> [/(subsetP tsb)|_].
     by case: color4P x_g.
@@ -454,7 +454,7 @@ Lemma stack_neq_infty e x : wf_color e -> wf_num e ->
 Proof. by move=> e_cwf e_nwf x_stack; rewrite wf_num_infty// stack_sccsF. Qed.
 
 Definition noblack_to_white e :=
-  forall x, x \in black e -> [disjoint successors x & whites e].
+  forall x, x \in black e -> [disjoint successors x & white e].
 
 Record wf_graph e := WfGraph {
   wf_gray_to_stack : {in gray e & stack e, forall x y,
@@ -483,7 +483,7 @@ Record pre_dfs (roots : {set V}) (e : env) := PreDfs {
 }.
 
 Lemma add_stack_gwf e w :
-  access_to e [set w] -> wf_color e -> wf_num e -> w \in whites e -> wf_graph e ->
+  access_to e [set w] -> wf_color e -> wf_num e -> w \in white e -> wf_graph e ->
   wf_graph (add_stack w e).
 Proof.
 move=> gray_to e_cwf e_nwf w_white [gs sg]; split.
@@ -502,7 +502,7 @@ by case: color4P y_stack x_gray.
 Qed.
 
 Lemma add_stack_pre e w :
-  access_to e [set w] -> wf_color e -> w \in whites e -> wf_graph e ->
+  access_to e [set w] -> wf_color e -> w \in white e -> wf_graph e ->
   access_to (add_stack w e) [set x in successors w].
 Proof.
 move=> gray_to e_wf w_white e_gwf.
@@ -523,13 +523,13 @@ Lemma nth_belast_small (z : V) p i : i < size p ->
   nth z (belast z p) i = nth z (z :: p) i.
 Proof. by move=> i_lt; rewrite nth_belast i_lt. Qed.
 
-Notation wedge e := (relfrom (pred_of_set (whites e)) edge).
+Notation wedge e := (relfrom (pred_of_set (white e)) edge).
 Definition wreach e x := [set y in connect (wedge e) x].
 
 Lemma mem_wreach e x : x \in wreach e x.
 Proof. by rewrite !inE connect0. Qed.
 
-Lemma Nwreach e x : x \notin whites e -> wreach e x = [set x].
+Lemma Nwreach e x : x \notin white e -> wreach e x = [set x].
 Proof.
 move=> xNwhite; apply/eqP; rewrite eqEsubset sub1set mem_wreach andbT.
 apply/subsetP=> y; rewrite !inE => /connectP [].
@@ -604,15 +604,15 @@ move=> e2_wf e12; pose n := subenvN e1 e2; exists (take n (stack e2)).
 by rewrite subenv_take.
 Qed.
 
-Lemma subenv_whites e1 e2 : subenv e1 e2 -> whites e2 \subset whites e1.
+Lemma subenv_white e1 e2 : subenv e1 e2 -> white e2 \subset white e1.
 Proof.
-by move=> e12; rewrite whitesE setCS (subenv_gray e12) setUS ?subenv_black.
+by move=> e12; rewrite whiteE setCS (subenv_gray e12) setUS ?subenv_black.
 Qed.
 
-Lemma new_whites e1 e2 : wf_color e2 -> subenv e1 e2 ->
-   whites e1 :\: whites e2 = black e2 :\: black e1.
+Lemma new_white e1 e2 : wf_color e2 -> subenv e1 e2 ->
+   white e1 :\: white e2 = black e2 :\: black e1.
 Proof.
-move=> e2_wf e12; rewrite whitesE -(subenv_gray e12) setDE setCK setIC -setDE.
+move=> e2_wf e12; rewrite whiteE -(subenv_gray e12) setDE setCK setIC -setDE.
 rewrite setDUl setDE setCU setIA setICr set0I set0U.
 rewrite setDUr (setIidPr _) // [_ :\: gray _](setDidPl _) ?subsetDl //.
 by apply/pred0P => y /=; case: color4P.
@@ -680,13 +680,13 @@ Qed.
 Record post_dfs (roots : {set V}) (e e' : env) (m : nat) := PostDfs {
   post_invariants : invariants e';
   post_subenv : subenv e e';
-  post_whites : whites e' = whites e :\: \bigcup_(x in roots) wreach e x;
+  post_white : white e' = white e :\: \bigcup_(x in roots) wreach e x;
   post_num : m = \min_(y in \bigcup_(x in roots) wreach e x)
                       @inord infty (num e' y);
 }.
 
 Definition dfs1_correct (dfs1 : V -> env -> nat * env) x e :=
-  (x \in whites e) -> pre_dfs [set x] e ->
+  (x \in white e) -> pre_dfs [set x] e ->
   let (m, e') := dfs1 x e in post_dfs [set x] e e' m.
 
 Definition dfs_correct (dfs : {set V} -> env -> nat * env) roots e :=
@@ -704,7 +704,7 @@ Proof. by move=> xNA; rewrite (setDidPl _) ?disjoints1. Qed.
 
 Lemma dfs_is_correct dfs1 dfsrec (roots : {set V}) e :
   (forall x, x \in roots -> dfs1_correct dfs1 x e) ->
-  (forall x, x \in roots -> forall e1, whites e1 \subset whites e ->
+  (forall x, x \in roots -> forall e1, white e1 \subset white e ->
          dfs_correct dfsrec (roots :\ x) e1) ->
   dfs_correct (dfs dfs1 dfsrec) roots e.
 Proof.
@@ -721,12 +721,12 @@ rewrite wf_num0 //; have [xw|xNw]/= := boolP (x \in _); last first.
   move: dfsrec_correct => /(_ _ (subxx _)).
   case: (dfsrec _ _) => [m2 e1].
   case; first exact: (pre_dfs_subroots (subD1set _ _)).
-  move=> [e1_wf e1_nwf e1_gwf Nbw1 sccs_e1] sube1 whites1 m2_min.
+  move=> [e1_wf e1_nwf e1_gwf Nbw1 sccs_e1] sube1 white1 m2_min.
   have [//|s1 s1_def sb] := subenv_stackP _ sube1.
   have e1_uniq := wf_uniq e1_wf.
   split=> //.
     rewrite -(setD1K x_root) big_setU1 ?setD11 //=.
-    by rewrite -setDDl whites1 Nwreach ?(subND1 xNw).
+    by rewrite -setDDl white1 Nwreach ?(subND1 xNw).
   rewrite -(setD1K x_root) big_setU1 ?setD11 // bigmin_setU /= m2_min.
   congr (minn _ _); rewrite Nwreach // big_set1 ord_num //.
   case: stackP xNw => // [x_stack|x_sccs] _; first exact/esym/subenv_num.
@@ -738,18 +738,18 @@ move: dfsrec_correct => /(_ e1).
 case: (dfsrec _ _) => [m2 e2] post_dfs {dfs1_is_correct dfs_is_correct}.
 have := post_dfs1 xw (pre_dfs_subroots _ pre).
 rewrite sub1set x_root => /(_ isT) {post_dfs1}.
-case=> [[e1_wf e1_cwf e1_gwf Nbw1 sccs_e1] sube1 whites1 m1_min].
+case=> [[e1_wf e1_cwf e1_gwf Nbw1 sccs_e1] sube1 white1 m1_min].
 have [//|s1 s1_def s1b] := subenv_stackP _ sube1.
 have e1_uniq := wf_uniq e1_wf.
-rewrite big_set1 in whites1 m1_min.
+rewrite big_set1 in white1 m1_min.
 case: post_dfs.
-- by rewrite subenv_whites.
+- by rewrite subenv_white.
 - split=> // y z; rewrite grayE !inE s1_def mem_cat.
   case: (y \in s1) (subsetP s1b y) => //= [->//|_ /andP[yNb ys]].
   move=> /andP[_ z_roots]; rewrite to_roots // grayE !inE.
   rewrite ys andbT; apply: contraNN yNb; apply/subsetP.
   by rewrite subenv_black.
-move=> [e2_wf e2_cwf e2_gwf Nbw2 sccs_e2] sube2 whites2 m2_min.
+move=> [e2_wf e2_cwf e2_gwf Nbw2 sccs_e2] sube2 white2 m2_min.
 have [//|s2 s2_def s2b] := subenv_stackP _ sube2.
 have e2_uniq := wf_uniq e2_wf.
 have split_wreach : \bigcup_(y in roots) wreach e y =
@@ -758,21 +758,21 @@ have split_wreach : \bigcup_(y in roots) wreach e y =
   rewrite !in_setU; have [//|/=Nxy] := boolP (_ \in wreach _ _).
   apply/bigcupP/bigcupP=> - [] z z_roots zy; exists z => //; last first.
     rewrite !inE in zy *; apply: connect_sub zy => u v /= /andP [uw uv].
-    by rewrite connect1 //= uv andbT; apply: subsetP uw; rewrite subenv_whites.
+    by rewrite connect1 //= uv andbT; apply: subsetP uw; rewrite subenv_white.
   apply: contraTT isT => Nzy; move: zy; rewrite !inE in  Nxy Nzy *.
   move=> /(connect_from (predC (connect (wedge e) x))) /= [t] /= [xtxy zt ty].
   move: zt; rewrite (@eq_connect _ _ (wedge e1)); last first.
-    by move=> u v /=; rewrite !inE /= whites1 !inE andbA.
+    by move=> u v /=; rewrite !inE /= white1 !inE andbA.
   case: (altP eqP) xtxy => /= [<-|neq_yt]; first by rewrite (negPf Nzy).
   by rewrite implybF negbK => /connect_trans /(_ ty); rewrite (negPf Nxy).
 split => //; first exact: subenv_trans sube2.
-  by rewrite whites2 whites1 split_wreach setDDl.
+  by rewrite white2 white1 split_wreach setDDl.
 rewrite m1_min m2_min split_wreach bigmin_setU /=.
 congr (minn (val _) _); apply: eq_bigr => y xy; apply/val_inj=> /=.
 rewrite !ord_num //.
 have /orP[ys|ysccs] : (y \in stack e1) || (y \in cover (sccs e1)).
-+ suff: y \notin whites e1 by case: color4P.
-  by rewrite whites1 inE xy.
++ suff: y \notin white e1 by case: color4P.
+  by rewrite white1 inE xy.
 + exact/esym/subenv_num.
 rewrite ?(num_inftyP _ _ _) //.
 by apply: (subsetP (subset_cover (subenv_sccs _))) ysccs.
@@ -792,10 +792,10 @@ case: post_dfs => //=.
     rewrite inE => /(@connect1 _ edge) //.
     by apply/connect_trans/access_to_x; rewrite ?set11.
     split=> //; do?[exact: add_stack_cwf|exact: add_stack_gwf|exact: add_stack_nwf].
-  move=> y /Nbw; rewrite whites_add_stack.
+  move=> y /Nbw; rewrite white_add_stack.
   rewrite ![[disjoint successors _ & _]]disjoint_sym.
   by apply/disjoint_trans/subsetDl.
-move=> [e1_wf e1_cwf e1_gwf Nbw1 black_sccs1] sube1 whites1 m_min.
+move=> [e1_wf e1_cwf e1_gwf Nbw1 black_sccs1] sube1 white1 m_min.
 have [//|s s_def sb] := subenv_stackP _ sube1.
 set s2 := rcons s x.
 have e1_uniq := @wf_uniq _ e1_wf.
@@ -817,7 +817,7 @@ have sx_subscc : is_subscc [set y in rcons s x].
   by rewrite (@wf_gray_to_stack e1) //; rewrite (subenv_gray_le sube1).
 have wreachex : wreach e x = x |: \bigcup_(y in [set y in successors x])
                           wreach (add_stack x e) y.
-  rewrite /wreach whites_add_stack.
+  rewrite /wreach white_add_stack.
   apply/eqP; rewrite eqEsubset subUset sub1set mem_wreach /=.
   apply/andP; split; last first.
     apply/bigcupsP => y; rewrite inE => xy; apply/subsetP=> z; rewrite !inE.
@@ -836,9 +836,9 @@ have m2_min : minn m m1 = \min_(y in wreach e x) @inord infty (num e1 y).
   rewrite wreachex bigmin_setU big_set1 //= /m -m_min; congr (minn _ _).
   rewrite (subenv_num sube1) ?mem_head//= ffunE/= eqxx.
   by rewrite inordK// ltnS sn_small.
-have succ_whiteF z : z \in successors x -> z \in whites e1 = false.
+have succ_whiteF z : z \in successors x -> z \in white e1 = false.
   move=> z_successor; apply/negbTE.
-  rewrite whites1 whites_add_stack !inE !negb_and !negbK.
+  rewrite white1 white_add_stack !inE !negb_and !negbK.
   by rewrite (appP bigcupP idP) //; exists z; rewrite !inE.
 case: ltnP => [m1_small|m1_big] //=.
   rewrite (minn_idPr _) 1?ltnW// in m2_min.
@@ -859,7 +859,7 @@ case: ltnP => [m1_small|m1_big] //=.
         rewrite ord_num // inordK//= lt0n wf_num0//.
         rewrite wreachex !inE => /predU1P[->|].
           by case: color4P x_stack. (* TODO: add this to ssrdone *)
-        by rewrite whites1 inE => ->.
+        by rewrite white1 inE => ->.
       apply: leq_trans (subenv_sn _ _ sube1); rewrite ?leqW //.
       by apply: add_stack_nwf.
     have [z [z_gray num_z y_to_z]] := wf_stack_to_gray e1_gwf x1_stack.
@@ -872,7 +872,7 @@ case: ltnP => [m1_small|m1_big] //=.
   - split=> //; first exact: add_black_cwf.
     + split => //.
       * move=> y /=.
-        by rewrite whites_add_black wf_num0// subND1//; case: color4P x_gray.
+        by rewrite white_add_black wf_num0// subND1//; case: color4P x_gray.
       * by move=> y /=; rewrite wf_num_infty.
       * by move=> y /= /wf_num_lt; apply.
       * by rewrite /= gray_add_black wf_sn// setUCA setUA setD1K.
@@ -889,7 +889,7 @@ case: ltnP => [m1_small|m1_big] //=.
       exists x'; split; rewrite 2?inE ?x'_gray ?andbT //.
       - by rewrite (leq_trans _ rank_x) 1?ltnW // rkx.
       - by rewrite (connect_trans y_to_x).
-    + move=> y; rewrite !inE whites_add_black.
+    + move=> y; rewrite !inE white_add_black.
       move=> /predU1P [->{y}|y_black]; last first.
         apply/pred0P=> z /=; rewrite 2!inE.
         have /pred0P /(_ z) /= := Nbw1 _ y_black.
@@ -910,7 +910,7 @@ case: ltnP => [m1_small|m1_big] //=.
       by case: color4P x'_gray.
   - apply/and5P; split => //=.
     + rewrite gray_add_black (subenv_gray sube1) gray_add_stack ?setU1K //.
-      by rewrite whites_grayF.
+      by rewrite white_grayF.
     + by rewrite (subset_trans (subenv_black sube1)) // subsetUr.
     + by rewrite -[sccs e]/(sccs (add_stack x e)) subenv_sccs.
     + apply/forall_inP => y y_stack; apply/eqP.
@@ -918,7 +918,7 @@ case: ltnP => [m1_small|m1_big] //=.
       by rewrite ifN//; apply: contraTneq xe_uniq => <- /=; rewrite y_stack.
     + apply/'exists_eqP/uniq_ex_drop; rewrite // s_def /=.
       by exists (rcons s x); rewrite cat_rcons.
-  - rewrite whites_add_black big_set1 wreachex whites1 whites_add_stack.
+  - rewrite white_add_black big_set1 wreachex white1 white_add_stack.
     by rewrite !setDDl setUA setUAC setUid.
   - by rewrite m2_min; congr val; apply: eq_bigl=> y; rewrite /= big_set1.
 (* post conditions *)
@@ -937,7 +937,7 @@ have scc_max : scc_of x \subset [set y in s2].
   move=> /connect1r [] // x' xx's2 /= /andP [x'_s2 x'y'] y'y.
   have xx' : gconnect x x'.
     by apply: connect_sub xx's2 => u v /= /andP[_]; apply: connect1.
-  have /or3P[] : [|| y' \in whites e1, y' \in cover (sccs e1)
+  have /or3P[] : [|| y' \in white e1, y' \in cover (sccs e1)
                    | y' \in stack e1] by case: color4P.
   - move: x'_s2; rewrite mem_rcons in_cons => /predU1P [eq_x'x|x_s].
       by rewrite succ_whiteF -?eq_x'x.
@@ -957,7 +957,7 @@ have scc_max : scc_of x \subset [set y in s2].
     have x'Nstack: x' \notin stack e.
       rewrite -(@uniq_catLR _ x' s2) ?mem_cat ?x'_s2 //.
       by rewrite cat_rcons -s_def wf_uniq.
-    have s2_whites: {subset s2 <= whites e}.
+    have s2_white: {subset s2 <= white e}.
       move=> z z_s2; have: z \notin cover (sccs e).
         apply/negP=> /(subsetP (subset_cover (subenv_sccs sube1))).
         suff: z \in stack e1 by case: color4P.
@@ -970,11 +970,11 @@ have scc_max : scc_of x \subset [set y in s2].
       rewrite !ffunE/= eqxx (negPf neq_y'x) leqNgt wf_num_lt//.
       by rewrite wf_num_infty//; case: color4P y'_stack.
     rewrite !inE (@connect_trans _ _ x') //; last first.
-       by rewrite connect1 /= ?s2_whites.
-    apply: connect_sub xx's2 => u v /= /andP[/s2_whites uw uv].
+       by rewrite connect1 /= ?s2_white.
+    apply: connect_sub xx's2 => u v /= /andP[/s2_white uw uv].
     by rewrite connect1 /= ?uw.
 have g1Nx : gray e1 :\ x = gray e.
-  by rewrite (subenv_gray sube1) gray_add_stack // setU1K // whites_grayF.
+  by rewrite (subenv_gray sube1) gray_add_stack // setU1K // white_grayF.
 have take_s : take (index x (stack e1)) (stack e1) = s.
   rewrite s_def index_cat /= eqxx addn0.
   rewrite (@uniq_catLR _ _ _ (x :: stack e)) -?s_def ?wf_uniq //.
@@ -988,7 +988,7 @@ split=> //.
 - split=> //.
   + by apply: add_sccs_wf=> //; rewrite take_s //.
   + split=> //=. (* TODO: generalize *)
-    * move=> y; rewrite whites_add_sccs// ?take_s//.
+    * move=> y; rewrite white_add_sccs// ?take_s//.
       rewrite set_infty_eq0 ?wf_num0//= => z; rewrite mem_rcons in_cons wf_num0//.
       by move=> /predU1P[->|/(subsetP sb)]; case: color4P x_stack.
     * move=> y; rewrite !take_s.
@@ -1048,7 +1048,7 @@ split=> //.
        exists z; split => //; first by rewrite -g1Nx !inE zDx.
        rewrite !ffunE ifN //= mem_rcons !inE (negPf zDx) /=.
        by apply/negP=> /(subsetP sb); case: color4P z_g.
-  + move=> y; rewrite !inE whites_add_sccs ?take_s //.
+  + move=> y; rewrite !inE white_add_sccs ?take_s //.
     move=> /predU1P [->|/Nbw1//]; apply/pred0P=> z //=.
     by have [/succ_whiteF->|] := boolP (z \in successors x).
   + rewrite sccs_add_sccs take_s //=; apply/setP=> scc.
@@ -1087,8 +1087,8 @@ split=> //.
     rewrite !ffunE /= !ifN => [->||] //.
     by apply: contra yNIr => /eqP->; rewrite mem_rcons inE eqxx.
   by apply/'exists_eqP; exists ord0; rewrite drop0.
-- rewrite whites_add_sccs ?take_s ?sb //.
-  by rewrite whites1 whites_add_stack big_set1 wreachex setDDl.
+- rewrite white_add_sccs ?take_s ?sb //.
+  by rewrite white1 white_add_stack big_set1 wreachex setDDl.
 - rewrite big_set1 /= take_s; apply/eqP; rewrite eqn_leq leq_ord andbT.
   rewrite [X in X <= _](_ : infty = @inord infty infty); last by rewrite inordK.
   apply/bigmin_geqP => y /= He.
@@ -1113,7 +1113,7 @@ split=> //.
 Qed.
 
 Theorem tarjan_rec_terminates n (roots : {set V}) e :
-  n >= #|whites e| * #|V|.+1 + #|roots| ->
+  n >= #|white e| * #|V|.+1 + #|roots| ->
   dfs_correct (tarjan_rec n) roots e.
 Proof.
 move=> n_ge; wlog ->: e n roots {n_ge} / roots = set0 => [noroot|]; last first.
@@ -1130,12 +1130,12 @@ elim: n => [|n IHn] in roots e n_ge *.
 move=> pre; rewrite /dfs_correct /=.
 apply: dfs_is_correct => //= x x_root.
   move=> x_white; apply: dfs1_is_correct => //; apply: IHn.
-  rewrite whites_add_stack cardsDS ?sub1set // cards1 subn1.
+  rewrite white_add_stack cardsDS ?sub1set // cards1 subn1.
   rewrite -ltnS (leq_trans _ n_ge) //.
   rewrite (@ltn_div2r #|V|.+1) ?divnMDl ?divn_small ?addn0 ?ltnS ?max_card //=.
   by rewrite prednK //; apply/card_gt0P; exists x.
-move=> e1 whites_e1; apply: IHn; rewrite -ltnS (leq_trans _ n_ge) //.
-have /subset_leq_card := whites_e1.
+move=> e1 white_e1; apply: IHn; rewrite -ltnS (leq_trans _ n_ge) //.
+have /subset_leq_card := white_e1.
 rewrite leq_eqVlt => /predU1P [->|lt_wh]; last first.
   by rewrite (@ltn_div2r #|V|.+1) ?divnMDl ?divn_small ?addn0 ?ltnS ?max_card.
 by rewrite ltn_add2l [X in _ < X](cardsD1 x) x_root.
@@ -1149,7 +1149,7 @@ case: tarjan_rec => [m e] [].
 - by rewrite ?leq_add ?leq_mul ?max_card.
 - do ![split=> //; rewrite /= ?cover0 ?gray0 ?set0D ?setU0 //];
     do ?by[do [move=> ?|move/setP=> ?]; rewrite ?gray0 inE].
-  + by move=> x; rewrite ffunE whitesE gray0 !inE eqxx.
+  + by move=> x; rewrite ffunE whiteE gray0 !inE eqxx.
   + by move=> x; rewrite ffunE inE eq_sym.
   + by move=> x; rewrite ffunE.
   + by rewrite cards0.
@@ -1160,7 +1160,7 @@ rewrite (eqP _ : \bigcup_(x in _) _ = setT) ?setDT => [whe ->|]; last first.
   rewrite -subTset; apply/subsetP=> y _; apply/bigcupP.
   by exists y; rewrite ?mem_wreach.
 have blacke : black e = setT.
-  move/eqP: whe; rewrite whitesE graye gray0 set0U.
+  move/eqP: whe; rewrite whiteE graye gray0 set0U.
   by rewrite -subset0 subCset setC0 subTset => /eqP.
 rewrite /black_gsccs blacke ?graye ?gray0 ?setTD ?set0U// in sccse stack_wf.
 have {sccse}sccse: sccs e = gsccs.
